WIP

coq-verification/src/Concrete/MM/Proofs.v
@@ -1,5 +1,6 @@
 Require Import Coq.Arith.PeanoNat.
 Require Import Coq.Lists.List.
+Require Import Coq.micromega.Lia.
 Require Import Coq.NArith.BinNat.
 Require Import Hafnium.AbstractModel.
 Require Import Hafnium.Concrete.Datatypes.
@@ -96,9 +97,9 @@ Section Proofs.
      state) *)
   Lemma mm_map_level_represents
         (conc : concrete_state)
-        t begin end_ attrs table level flags ppool :
+        begin end_ pa attrs table level flags ppool :
     (snd (fst (mm_map_level
-                 conc t begin end_ attrs table level flags ppool))) = conc.
+                 conc begin end_ pa attrs table level flags ppool))) = conc.
   Proof.
     autounfold; cbv [mm_map_level].
     repeat match goal with
@@ -110,19 +111,103 @@ Section Proofs.
            end.
   Qed.
 
+  Lemma mm_map_level_table_attrs conc begin end_ pa attrs table level
+        flags ppool :
+    let ret :=
+        mm_map_level conc begin end_ pa attrs table level flags ppool in
+    let success := fst (fst (fst ret)) in
+    let table := snd (fst (fst ret)) in
+    let conc' := snd (fst ret) in
+    let ppool' := snd ret in
+    let begin : nat := mm_index begin level in
+    let end_ : nat := mm_index end_ level in
+    has_uniform_attrs conc'.(ptable_deref) table level attrs begin end_.
+  Admitted.
+
   (* placeholder; later there will be actual expressions for the new abstract
      states *)
   Axiom TODO : @abstract_state paddr_t nat.
 
+  (* TODO: we know that all the mm_map_level steps succeed because we
+  know that the whole thing succeeds. But how do we use that in the
+  invariant? *)
   Definition mm_map_root_loop_invariant
-             start_abst start_conc t_ptr start_begin attrs root_level
+             start_abst start_conc t_ptrs start_begin attrs root_level
              (state : concrete_state * ptable_addr_t * size_t * bool * mpool)
     : Prop :=
     let '(s, begin, table_index, failed, ppool) := state in
     let index := mm_index begin root_level in
-    represents
-      (abstract_reassign_pointer start_abst start_conc t_ptr attrs start_begin index)
-      s.
+    table_index = index /\
+    (failed = true \/
+     represents
+       (fold_right
+          (fun t_ptr abst =>
+             abstract_reassign_pointer abst start_conc t_ptr attrs start_begin index)
+          start_abst
+          (firstn table_index t_ptrs))
+       s).
+
+  (* TODO: move *)
+  Lemma N_lnot_0_r a : N.lnot a 0 = a.
+  Proof. destruct a; reflexivity. Qed.
+
+  (* TODO: move *)
+  Lemma N_div2_lnot a n : N.div2 (N.lnot a n) = N.lnot (N.div2 a) (N.pred n).
+  Admitted. (* TODO *)
+    
+  (* TODO: move *)
+  Lemma N_lnot_shiftr a n m : ((N.lnot a n >> m) = N.lnot (a >> m) (n - m))%N.
+  Proof.
+    rewrite <-(Nnat.N2Nat.id m).
+    induction (N.to_nat m).
+    { rewrite !N.shiftr_0_r.
+      rewrite N.sub_0_r. reflexivity. }
+    { rewrite Nnat.Nat2N.inj_succ.
+      rewrite !N.shiftr_succ_r.
+      rewrite N.sub_succ_r.
+      rewrite <-N_div2_lnot.
+      solver. }
+  Qed.
+
+  (* TODO: move *)
+  Lemma N_log2_add_shiftl_1 a b : (b <= N.log2 (a + (1 << b)))%N.
+  Admitted. (* TODO *)
+
+  (* TODO: include 0 < PAGE_BITS axiom *)
+  Lemma mm_start_of_next_block_shift a level :
+    (0 < PAGE_BITS)%N ->
+    (mm_start_of_next_block a (mm_entry_size level)
+                            >> (PAGE_BITS + level * PAGE_LEVEL_BITS))%N =
+    ((a >> (PAGE_BITS + level * PAGE_LEVEL_BITS)) + 1)%N.
+  Proof.
+    intros.
+    cbv [mm_start_of_next_block mm_entry_size].
+    rewrite !Nnat.N2Nat.id, N.shiftr_land, N_lnot_shiftr.
+    rewrite N.shiftr_eq_0 with (a:=((_ << _) - 1)%N) by
+        (rewrite N.sub_1_r, N.shiftl_1_l, N.log2_pred_pow2 by lia; lia).
+    rewrite N.lnot_0_l.
+    match goal with
+    | |- context [((_ + (_ << ?x)) >> ?x)%N] =>
+      pose proof (N_log2_add_shiftl_1 a x);
+        assert ((1 << x) <> 0)%N by (rewrite N.shiftl_eq_0_iff; lia)
+    end.
+    rewrite N.land_ones_low by (rewrite N.log2_shiftr, N.size_log2 by lia; lia).
+    rewrite !N.shiftr_div_pow2, !N.shiftl_mul_pow2.
+    rewrite N.div_add by (apply N.pow_nonzero; lia).
+    lia.
+  Qed.
+
+  Lemma mm_index_start_of_next_block a level :
+    mm_index (mm_start_of_next_block a (mm_entry_size level)) level
+    = S (mm_index a level).
+  Proof.
+    cbv [mm_index].
+    rewrite mm_start_of_next_block_shift.
+    remember ((1 << PAGE_LEVEL_BITS) - 1)%N as mask.
+    remember (PAGE_BITS + level * PAGE_LEVEL_BITS)%N as B.
+    (* TODO: won't be *hard*, but will be annoying. Will likely require a
+       precondition in terms of mm_level_end. *)
+  Admitted.
 
   (* TODO:
      This proof says only that if success = true and commit = true
@@ -140,32 +225,54 @@ Section Proofs.
     let ppool' := snd ret in
     let conc' := snd (fst ret) in
     let success := fst (fst ret) in
-    let t_ptr := ptable_pointer_from_address t.(root) in
+    let t_ptrs := mm_page_table_from_pa t.(root) in
     let begin_index := mm_index begin root_level in
     let end_index := mm_index end_ root_level in
     success = true ->
     ((flags & MM_FLAG_COMMIT) != 0)%N = true ->
     (begin <= end_)%N ->
+    end_index < length t_ptrs ->
     forall abst,
       represents abst conc ->
-      represents (abstract_reassign_pointer
-                    abst conc t_ptr attrs begin_index end_index) conc'.
+      represents (fold_right
+                    (fun t_ptr abst =>
+                       abstract_reassign_pointer
+                         abst conc t_ptr attrs begin_index end_index)
+                    abst t_ptrs)
+                 conc'.
   Proof.
     cbv zeta. cbv [mm_map_root].
     simplify.
 
-    let t_ptr := constr:(ptable_pointer_from_address t.(root)) in
+    let t_ptrs := constr:(mm_page_table_from_pa t.(root)) in
     let start_begin := constr:(mm_index begin root_level) in
     match goal with
     | |- context [@while_loop _ ?iter ?cond ?start ?body] =>
       assert (mm_map_root_loop_invariant
-                abst conc t_ptr start_begin attrs root_level
+                abst conc t_ptrs start_begin attrs root_level
                 (@while_loop _ iter cond start body));
-        [ apply while_loop_invariant | ];
-        cbv [mm_map_root_loop_invariant] in *; simplify
+        [ apply while_loop_invariant | ]
+    end;
+      cbv [mm_map_root_loop_invariant] in *; simplify;
+        repeat inversion_bool;
+        rewrite ?mm_map_level_represents.
+    { rewrite mm_index_start_of_next_block; reflexivity. }
+    { rewrite mm_index_start_of_next_block; reflexivity. }
+    { right.
+      cbn [firstn fold_right].
+      rewrite ?mm_map_level_represents.
+        cbv [mm_map_root_loop_invariant] in *; simplify.
+        right.
+          rewrite ?mm_map_level_represents
     end.
-    3:admit. (* TODO: proof that if begin and end are the same then has_uniform_attrs is trivially true *)
-    all:rewrite ?mm_map_level_represents.
+    Check while_loop_invariant.
+    { (* TODO: in this case, the map_level step failed, so we can't have returned success. *)
+      
+      Check reassign_pointer_represents.
+      Print mm_page_table_from_pa.
+      Check ptable_pointer_from_address.
+      SearchAbout s.
+    3:rewrite abstract_reassign_pointer_trivial; solver.
     1-2: admit. (* mm_map_level layer *)
 
     match goal with
